

# Converting a CFG into a PDA

## Converting a CFG into a PDA

Let  $G = (\Sigma, N, S, P)$  be a CFG. Then, define a nondeterministic PDA,  $M = (Q, \Sigma, \Gamma, \delta, q_0, S, \emptyset)$ , as follows, where **acceptance is by empty stack**:

- $Q = \{q_0, q_1\}$ , where  $q_0$  is the start state,
- $\Sigma$  is the same for  $G$  and  $M$ ,
- $S$  = the stack start symbol (bottom of stack symbol),
- $\Gamma = \Sigma \cup N$ ,
- $\delta$ : is the transition function over  $Q \times \Sigma \times \Gamma \rightarrow Q \times \Gamma^*$ , defined as follows, where  $x \in \Sigma, A \in N$ :
  - $\delta(q_0, \varepsilon, \varepsilon) = \{(q_1, S)\}$
  - $\delta(q_1, x, x) = \{(q_1, \varepsilon)\}$  for each  $x \in \Sigma$
  - $\delta(q_1, \varepsilon, A) = \{(q_1, \alpha)\}$  for each production  $A \rightarrow \alpha$

# Example

Design a push-down automaton,  $M$ , to recognize the language generated by following context-free grammar:

$$E \rightarrow T \mid E * E \mid E + E \mid (E)$$

$$T \rightarrow a \mid b \mid Ta \mid Tb \mid T0 \mid T1$$

# Note

$$E \rightarrow T \mid E * E \mid E + E \mid (E)$$

is the same as:

$$E \rightarrow T$$

$$E \rightarrow E * E$$

$$E \rightarrow E + E$$

$$E \rightarrow (E)$$

## Example Solution

$$E \rightarrow T \mid E * E \mid E + E \mid (E)$$

$$T \rightarrow a \mid b \mid Ta \mid Tb \mid T0 \mid T1$$

Define a nondeterministic PDA,

$M = (\{q_0, q_1\}, \Sigma, \Gamma, \delta, q_0, E, \emptyset)$ , as follows,  
where acceptance is by *empty stack*:

$$N = \{E, T\}$$

$$\Sigma = \{a, b, 0, 1, (, ), +, *\}$$

$$\Gamma = \{a, b, 0, 1, (, ), +, *, E, T\}$$

## Example Solution Continued

$$E \rightarrow T \mid E * E \mid E + E \mid (E)$$

$$T \rightarrow a \mid b \mid Ta \mid Tb \mid T0 \mid T1$$

$\delta$  is defined as follows:

$$\delta(q_0, \varepsilon, \varepsilon) = \{(q_1, E)\}$$

$$\delta(q_1, \varepsilon, E) = \{(q_1, T), (q_1, E + E), (q_1, E * E), (q_1, (E))\}$$

$$\delta(q_1, \varepsilon, T) = \{(q_1, a), (q_1, b), (q_1, Ta), (q_1, Tb), (q_1, T0), (q_1, T1)\}$$

$$\delta(q_1, a, a) = \{(q_1, \varepsilon)\}$$

$$\delta(q_1, b, b) = \{(q_1, \varepsilon)\}$$

$$\delta(q_1, 0, 0) = \{(q_1, \varepsilon)\}$$

$$\delta(q_1, 1, 1) = \{(q_1, \varepsilon)\}$$

$$\delta(q_1, +, +) = \{(q_1, \varepsilon)\}$$

$$\delta(q_1, *, *) = \{(q_1, \varepsilon)\}$$

$$\delta(q_1, '(', '(') = \{(q_1, \varepsilon)\}$$

$$\delta(q_1, ')', ')') = \{(q_1, \varepsilon)\}$$

$$N = \{E, T\}$$

$$\Sigma = \{a, b, 0, 1, (, ), +, *\}$$